# uniproof

6 == 3 * 2

6 == 3 + 2 + 1

7 == 3 + (2*2)

7 == 3 + (2 + 2)

7 == 3 + (2^2)

6 + 1 is every compiling operation of 3 and 2 $ 2

6 is the first x + (x+1) (()+1) in 3 span

AND ends with + 1

AND it’s a single tack on

IF use +1 to get from 6 to 7, fundamental connection to derived by basic operation must be *
⇒ 42

AND 2 and 4 are endpoints range 2,..., 4

3 + 4 == 7

2 ^ 3 == 8

3 ^ 2 == 9 

7, 8, 9

Emerge from manipulation on key intermediates 2, 3, 4

2 and 3 being crucial dimension span adjacents make sense to be reverse ordered exponentials

AND 6, 7 can be differentially decomposed as 2 * 3 and 3 + 4 respectively, coincidentally can individually be sequence-proportioned into the bounds of the ratio range
